\documentclass[a4paper,10pt,fleqn]{article}
\usepackage{fancyhdr}
\usepackage{amsmath}
\usepackage[margin=1.8cm]{geometry}
\usepackage{ulem} %used for strikeout


%Use custom fitch style proof package http://www.phil.cam.ac.uk/teaching_staff/Smith/LaTeX/fitch.html http://folk.uio.no/johanw/FitchSty.html
%Guide here http://angasm.org/papers/fitch/
\usepackage{fitch}

\newcommand{\danspagestyle}
{
%blank header & footer
\fancyhf{}
%set footer and header values
%\lhead{\textsf{Imperial College London}}
\rhead{Logic \& AI Programming}
\cfoot{page \thepage}
\rfoot{Daniel Liew}
}
\pagestyle{fancy}
\danspagestyle
%remove header ruler
\renewcommand{\headrulewidth}{0pt}
%set gap between paragraphs
\setlength{\parskip}{1ex plus0.5ex minus0.1ex}

%modify plain style so first pages of chapter get correct style.
\fancypagestyle{plain}{
\danspagestyle
}

%custom commands
\input{rules}


\newtheorem{lem}{Lemma}

\usepackage[pdfborder={0 0 0},colorlinks=true]{hyperref}

\setlength{\parindent}{0cm} % remove paragraph indentation

%opening
\title{Logic Inference proofs}
\author{Daniel Liew}

\begin{document}
\maketitle
\tableofcontents

\section{Introduction}
This contains various induction style proofs. There are probably mistakes. The source code for this \LaTeX document is available at \url{https://github.com/delcypher/propositional-logic-induction-proofs}. Feel free to fix mistakes.

\section{Equivalences}

	\subsection{ \texorpdfstring{ $ A \to B  \equiv \lnot A \lor B $ }{A implies B} }
	\label{sec:aimpliesB}
	$A \to B \vdash \lnot A \lor B$
	\begin{equation*}
		\begin{fitch}
		\fa A \to B & \giv  \\
			\fa\fh \lnot( \lnot A \lor B ) & \ass \\
				\fa\fa\fh A & \ass \\ %3
				\fa\fa\fa B & \arrowE{1}{3} \\ %4 
				\fa\fa\fa \lnot A \lor B & \orI{4} \\ %5
			\fa\fa \lnot A & \raa{3}{2}{5} \\ %6 
			\fa\fa \lnot A \lor B & \orI{6} \\ %7
		\fa \lnot A \lor B & \raa{2}{7}{2} \\
		\end{fitch}
	\end{equation*}

	$\lnot A \lor B \vdash A \to B$
	\begin{equation*}
		\begin{fitch}
		\fa \lnot A \lor B & \giv \\ %1
			\fa\fh A & \ass \\ %2 
			\fa\fa \lnot\lnot A & Double Negation Rule{3} \\ %3 
			\fa\fa B & \orE{1}{3}\\ %4
		\fa A \to B & \arrowI{2}{4} %5
		\end{fitch}
	\end{equation*}

	\subsection{ \texorpdfstring{$ A \to B \equiv \lnot B \to \lnot A $}{A implies B}}
	\label{sec:aimpliesB_contra}
	$  A \to B \vdash \lnot B \to \lnot A$
	\begin{equation*}
		\begin{fitch}
		\fa A \to B & \giv \\ %1
			\fa\fh \lnot B & \ass \\ %2 
				\fa\fa\fh A & \ass \\ %3 
				\fa\fa\fa B & \arrowE{1}{3} \\ %4
			\fa\fa \lnot A & \raa{3}{2}{4} \\ %5
		\fa \lnot B \to \lnot A & \arrowI{2}{5} \\ %6
		\end{fitch}
	\end{equation*}

	$ \lnot B \to \lnot A \vdash A \to B $
	\begin{equation*}
		\begin{fitch}
		\fa \lnot B \to \lnot A & \giv \\ %1
			\fa\fh A & \ass \\ %2 
				\fa\fa\fh \lnot B & \ass \\ %3 
				\fa\fa\fa \lnot A & \arrowE{1}{3} \\ %4
			\fa\fa B & \raa{3}{2}{4} \\ %5
		\fa A \to B & \arrowI{2}{5} \\ %6
		\end{fitch}
	\end{equation*}

	\subsection{DeMorgan's rule: \texorpdfstring{ $ \lnot ( A \lor B) \equiv \lnot A \land \lnot B$}{DeMorgan}}
	\label{sec:demorganor}
	$\lnot ( A \lor B) \vdash \lnot A \land \lnot B$
		\begin{equation*}
		\begin{fitch}
		\fa \lnot(A \lor B) & \giv \\ %1
			\fa\fh A & \ass \\ %2
			\fa\fa A \lor B & \orI{2} \\ %3
		\fa \lnot A & \raa{2}{1}{3} \\ %4
			\fa\fh B & \ass \\ %5
			\fa\fa A \lor B & \orI{5} \\ %6
		\fa \lnot B & \raa{5}{1}{5} \\  %7
		\fa \lnot A \land \lnot B & \andI{4}{7}
		\end{fitch}
	\end{equation*}

	$\lnot A \land \lnot B \vdash  \lnot ( A \lor B)$
	\begin{equation*}
		\begin{fitch}
		\fa \lnot A \land \lnot B & \giv \\ %1
			\fa\fh A \lor B & \ass \\ %2
			\fa\fa \lnot B & \andE{1} \\ %3
			\fa\fa A & \orE{2}{3} \\ %4
			\fa\fa \lnot A & \andE{1} \\ %5
		\fa \lnot(A \lor B) & \raa{2}{4}{5} \\ %6
		\end{fitch}
	\end{equation*}

	\subsection{DeMorgan's rule: \texorpdfstring{ $ \lnot( A \land B) \equiv \lnot A \lor \lnot B $}{DeMorgan}}
	$ \lnot( A \land B) \vdash \lnot A \lor \lnot B$
	\begin{equation*}
		\begin{fitch}
		\fa \lnot (A \land B) & \giv \\ %1
			\fa\fh \lnot (\lnot A \lor \lnot B) & \ass \\ %2
				\fa\fa\fh \lnot B & \ass \\ %3
				\fa\fa\fa \lnot A \lor \lnot B & \orI{3} \\ %4
			\fa\fa B & \raa{3}{2}{4} \\ %5
				\fa\fa\fh \lnot A & \ass \\ %6
				\fa\fa\fa \lnot A \lor \lnot B & \orI{6} \\ %7
			\fa\fa A & \raa{6}{2}{7} \\ %8
			\fa\fa A \land B & \andI{5}{8} \\ %9
		\fa \lnot A \lor \lnot B & \raa{2}{1}{9}
		\end{fitch}
	\end{equation*}

	$  \lnot A \lor \lnot B  \vdash\lnot( A \land B) $
	\begin{equation*}
		\begin{fitch}
		\fa \lnot A \lor \lnot B & \giv \\ %1
			\fa\fh A \land B & \ass \\ %2
			\fa\fa A & \andE{2} \\ %3
			\fa\fa \lnot B & \orE{1}{3} \\ %4
			\fa\fa B & \andE{2} \\ %5
		\fa \lnot(A \land B) & \raa{2}{4}{5}
		\end{fitch}
	\end{equation*}

	\subsection{Distributive rule: \texorpdfstring{$ A \lor (B \land C) \equiv (A \lor B) \land ( A \lor C) $}{Distributive}}
	$  A \lor (B \land C) \vdash  (A \lor B) \land ( A \lor C) $
	\begin{equation*}
		\begin{fitch}
			\fa  A \lor (B \land C) & \giv \\ %1
				\fa\fh \lnot A & \ass \\ %2
				\fa\fa B \land C & \orE{1}{2} \\ %3
				\fa\fa B & \andE{3} \\ %4
			\fa \lnot A \to B & \arrowI{2}{4} \\ %5
			\fa A \lor B & Apply lemma \ref{sec:aimpliesB} to 5 \\ %6
				\fa\fh \lnot A & \ass \\ %7
				\fa\fa B \land C & \orE{1}{7} \\ %8
				\fa\fa C & \andE{8} \\ %9
			\fa \lnot A \to C & \arrowI{7}{9} \\ %10
			\fa A \lor C & Apply lemma \ref{sec:aimpliesB} to 10 \\ %11
			\fa (A \lor B) \land (A \lor C) & \andI{6}{11} \\
		\end{fitch}
	\end{equation*}

	$  (A \lor B) \land ( A \lor C)  \vdash  A \lor (B \land C) $
	\begin{equation*}
		\begin{fitch}
			\fa (A \lor B) \land ( A \lor C)  & \giv \\ %1
			\fa (A \lor B) & \andE{1} \\ %2
			\fa (A \lor C) & \andE{1} \\ %3
				\fa\fh \lnot A & \ass \\ %4
				\fa\fa B & \orE{2}{4} \\ %5
				\fa\fa C & \orE{3}{4} \\ %6
				\fa\fa B \land C & \andI{5}{6} \\ %7
			\fa \lnot A \to (B \land C) & \arrowI{4}{7} \\ %8
			\fa A \lor (B \land C) & Apply lemma \ref{sec:aimpliesB} to 8 \\
		\end{fitch}
	\end{equation*}

	\subsection{Distributive rule: \texorpdfstring{$ A \land (B \lor C) \equiv (A \land B ) \lor (A \land C) $}{Distributive}}
	$A \land (B \lor C) \vdash (A \land B ) \lor (A \land C) $
	\begin{equation*}
		\begin{fitch}
			\fa A \land (B \lor C)  & \giv \\ %1
				\fa\fh \lnot ( (A \land B) \lor (A \land C) ) & \ass \\ %2
				\fa\fa A & \andE{1} \\ %3
				\fa\fa B \lor C & \andE{1} \\ %4
				\fa\fa \lnot(A \land B) \land \lnot(A \land C) & Apply lemma \ref{sec:demorganor} to 2\\ %5
				\fa\fa \lnot(A \land B) & \andE{5} \\ %6
				\fa\fa \lnot(A \land C) & \andE{5} \\ %7
					\fa\fa\fh \lnot C & \ass \\ %8
					\fa\fa\fa B & \orE{4}{8} \\ %9
					\fa\fa\fa A \land B & \andI{3}{9} \\ %10
				\fa\fa C & \raa{8}{6}{10} \\ %11
				\fa\fa A \land C & \andI{3}{11} \\ %12
			\fa (A \land B) \lor (A \land C) & \raa{2}{7}{12} \\ %13
		\end{fitch}
	\end{equation*}
	
	$ (A \land B ) \lor (A \land C)  \vdash A \land (B \lor C) $
	\begin{equation*}
		\begin{fitch}
			\fa (A \land B ) \lor (A \land C)  & \giv \\ %1
				\fa\fh \lnot A & \ass \\ %2
					\fa\fa\fh \lnot(A \land B) & \ass \\ %3
					\fa\fa\fa A \land C & \orE{1}{3} \\ %4
					\fa\fa\fa A & \andE{4} \\ %5
				\fa\fa A \land B & \raa{3}{2}{5} \\ %6
				\fa\fa A & \andE{6} \\ %7
			\fa A & \raa{2}{2}{6} \\ %8
				\fa\fh \lnot (B \lor C) & \ass \\ %9
					\fa\fa\fh \lnot(A \land C) & \ass \\ %10
					\fa\fa\fa A \land B & \orE{1}{10} \\ %11
					\fa\fa\fa B & \andE{11} \\ %12
					\fa\fa\fa B \lor C & \orI{12} \\ %13
				\fa\fa A \land C & \raa{10}{9}{13} \\ %14
				\fa\fa C & \andE{14} \\ %15
				\fa\fa B \lor C & \orI{15} \\ %16
			\fa B \lor C & \raa{9}{9}{16} \\ % 17
			\fa A \land (B \lor C) & \andI{8}{16} \\ % 18
		\end{fitch}
	\end{equation*}

	\subsection{\texorpdfstring{Commutative rule: $A \lor B \equiv B \lor A$ }{Commutative}}
	$ A \lor B \vdash B \lor A$
	\begin{equation*}
		\begin{fitch}
			\fa A \lor B  & \giv \\ %1
				\fa\fh \lnot (B \lor A)  & \ass \\ %2
					\fa\fa\fh \lnot B & \ass \\ %3
					\fa\fa\fa A & \orE{1}{3} \\ %4
					\fa\fa\fa B \lor A & \orI{4} \\ %5
				\fa\fa B & \raa{3}{2}{5} \\ %6
				\fa\fa B \lor A & \orI{6} \\ %7
			\fa B \lor A & \raa{2}{2}{7} \\ %8
		\end{fitch}
	\end{equation*}

	$ B \lor A \vdash A \lor B$ \\
	Proof is the same as above except with $A$ and $B$ swapped around.

	\subsection{\texorpdfstring{Commutative rule: $A \land B \equiv B \land A$}{Commutative}}
	$A \land B \vdash B \land A$
	\begin{equation*}
		\begin{fitch}
			\fa A \land B  & \giv \\ %1
			\fa B & \andE{1} \\ %2
			\fa A & \andE{1} \\ %3
			\fa B \land A & \andI{2}{3} \\ %4
		\end{fitch}
	\end{equation*}

	$B \land A \vdash A \land B$\\
	Proof is the same as above except with $A$ and $B$ swapped around.

	\subsection{\texorpdfstring{Associative rule: $(A \lor B) \lor C \equiv A \lor (B \lor C) $}{Associative}}
	These proofs are a little convoluted. But I don't have anything better.\\
	$(A \lor B) \lor C \vdash A \lor (B \lor C) $
	\begin{equation*}
		\begin{fitch}
			\fa (A \lor B) \lor C & \giv \\ %1
				\fa\fh \lnot ( A \lor (B \lor C) ) & \ass \\ %2
					\fa\fa\fh \lnot C & \ass \\ %3
					\fa\fa\fa (A \lor B) & \orE{1}{3} \\ %4
						\fa\fa\fa\fh \lnot A & \ass \\ %5
						\fa\fa\fa\fa  B & \orE{4}{5} \\ %6
						\fa\fa\fa\fa (B \lor C) & \orI{6} \\ %7
						\fa\fa\fa\fa A \lor ( B \lor C) & \orI{7} \\ %8
					\fa\fa\fa A & \raa{5}{2}{8} \\ %9
					\fa\fa\fa A \lor ( B \lor C) & \orI{9} \\ %10
				\fa C & \raa{3}{2}{10} \\ %11
				\fa (B \lor C ) & \orI{11} \\ %12
				\fa A \lor ( B \lor C) & \orI{12} \\ %13
			A \lor ( B \lor C) & \raa{2}{2}{13} \\ %14					
		\end{fitch}
	\end{equation*}

	$A \lor (B \lor C) \vdash (A \lor B) \lor C$
	\begin{equation*}
		\begin{fitch}
			\fa A \lor (B \lor C) & \giv \\ %1
				\fa\fh \lnot ( (A \lor B) \lor C ) & \ass \\ %2
					\fa\fa\fh \lnot A & \ass \\ %3
					\fa\fa\fa B \lor C & \orE{1}{3} \\ %4
						\fa\fa\fa\fh \lnot C & \ass \\ %5
						\fa\fa\fa\fa B & \orE{4}{5} \\ %6
						\fa\fa\fa\fa (A \lor B) & \orI{6} \\ %7
						\fa\fa\fa\fa (A \lor B) \lor C & \orI{7} \\ %8
					\fa\fa\fa C & \raa{5}{2}{8} \\ %9
					\fa\fa\fa (A \lor B) \lor C & \orI{9} \\ %10
				\fa\fa A & \raa{2}{2}{10} \\ %11
				\fa\fa (A \lor B) & \orI{11} \\ %12
				\fa\fa (A \lor B) \lor C & \orI{12} \\ %13
			\fa  (A \lor B) \lor C  & \raa{2}{2}{13} \\ %14
		\end{fitch}
	\end{equation*}

	\subsection{\texorpdfstring{Associative rule: $(A \land B) \land C \equiv A \land (B \land C) $}{Associative}}
	$ (A \land B) \land C \vdash A \land (B \land C)$
	\begin{equation*}
		\begin{fitch}
			\fa (A \land B) \land C & \giv \\ %1
			\fa C & \andE{1} \\ %2
			\fa A \land B  & \andE{2} \\ %3
			\fa B & \andE{3} \\ %4
			\fa (B \land C) & \andI{2}{4} \\ %5
			\fa A & \andE{3} \\ %6
			\fa A \land ( B \land C) & \andI{6}{5}
		\end{fitch}
	\end{equation*}

	$ A \land (B \land C) \vdash  (A \land B) \land C$
	\begin{equation*}
		\begin{fitch}
			\fa A \land (B \land C) & \giv \\ %1
			\fa A & \andE{1} \\ %2
			\fa B \land C & \andE{1} \\ %3
			\fa B & \andE{3} \\ %4
			\fa (A \land B) & \andI{2}{4} \\ %5
			\fa C & \andE{3} \\ %6
			\fa (A \land B) \land C & \andI{5}{6} \\ %7
		\end{fitch}
	\end{equation*}

	\subsection{\texorpdfstring{Double Negation rule: $ \lnot \lnot A \equiv A $}{Double Negation}}
	$ \lnot \lnot A \vdash A$
	\begin{equation*}
		\begin{fitch}
			\fa \lnot ( \lnot A ) & \giv \\ %1
				\fa\fh ( \lnot A) & \ass \\ %2
			\fa A & \raa{2}{1}{2} \\ %3	
		\end{fitch}
	\end{equation*}

	$ A \vdash \lnot \lnot A $
	\begin{equation*}
		\begin{fitch}
			\fa A & \giv \\ %1
				\fa\fh \lnot A & \ass \\ %2
			\fa \lnot (\lnot A ) & \raa{2}{1}{2} \\ %3
	
		\end{fitch}
	\end{equation*}
	


	

\section{Additional inference rules}

	\subsection{Law of excluded middle: \texorpdfstring{$ \vdash A \lor \lnot A$}{} }
	\begin{equation*}
		\begin{fitch}
				\fa\fh \lnot( A \lor \lnot A) & \ass \\ %1
				\fa\fa \lnot A \land A & Apply lemma \ref{sec:demorganor} to 1 \\ %2
				\fa\fa \lnot A & \andE{2} \\ %3
				\fa\fa A & \andE{2} \\ %4
			\fa A \lor \lnot A & \raa{1}{3}{4} \\ %5
		\end{fitch}
	\end{equation*}
	
	
	\subsection{Proof By Cases: \texorpdfstring{$ A \lor B, A \to C, B \to C \vdash C$}{} }
	\begin{equation*}
		\begin{fitch}
			\fa A \lor B & \giv \\ %1
			\fa A \to C & \giv \\ %2
			\fa B \to C & \giv \\ %3
				\fa\fh \lnot C & \ass \\ %4
					\fa\fa\fh \lnot A & \ass \\ %5
					\fa\fa\fa B & \orE{1}{5} \\ %6
					\fa\fa\fa C & \arrowE{3}{6} \\ %7
				\fa\fa A & \raa{5}{2}{7} \\ %8
				\fa\fa C & \arrowE{2}{8} \\ %9
			\fa C & \raa{4}{4}{9} \\ %10
		\end{fitch}
	\end{equation*}

	\subsection{Modus Tollens: \texorpdfstring{$ A \to B , \lnot B \vdash \lnot A$}{} }
	\begin{equation*}
		\begin{fitch}
			\fa A \to B & \giv \\ %1
			\fa \lnot B & \giv \\ %2
				\fa\fh A & \ass \\ %3
				\fa\fa B & \arrowE{1}{3} \\ %4
			\fa \lnot A & \raa{3}{2}{4} \\ %5
		\end{fitch}
	\end{equation*}

	\subsection{Contraposition: \texorpdfstring{$ A \to B \vdash \lnot B \to \lnot A$}{} }
	See section \ref{sec:aimpliesB_contra}.

	\subsection{Dilema: \texorpdfstring{$ A \to B , \lnot A \to B \vdash B$}{} }
	\begin{equation*}
		\begin{fitch}
			\fa A \to B & \giv \\ %1
			\fa \lnot A \to B & \giv \\ %2
				\fa\fh \lnot B & \ass \\ %3
					\fa\fa\fh A & \ass \\ %4
					\fa\fa\fa B & \arrowE{1}{4} \\ %5
				\fa\fa \lnot A & \raa{4}{3}{5} \\ %6
				\fa\fa B & \arrowE{2}{6} \\ %7
			\fa B & \raa{3}{3}{7} \\ %8
	
		\end{fitch}
	\end{equation*}
	
	
	



\section{Predicate Logic Equivalences}
  \subsection{DeMorgan's rule: \texorpdfstring{ $ \lnot \exists X p(X) \equiv \forall X \lnot p(X) $}{DeMorgan}}
	
	$ \lnot \exists X p(X) \vdash \forall X \lnot p(X) $
		\begin{equation*}
		\begin{fitch}
  		\fa \lnot \exists X p(X) & \giv \\ %1
  			\fa\fh p(a) & \ass \\ %2
        \fa\fa \exists X p(X) & \existsI{2} \\ %3
      \fa \lnot p(a) & \raa{2}{1}{3}  \\ %4
      \fa \forall X \lnot p(X) & \forallI{4} \\%5
		\end{fitch}
	\end{equation*}

	$ \forall X \lnot p(X) \vdash \lnot \exists X p(X) $
	\begin{equation*}
		\begin{fitch}
		  \fa \forall X \lnot p(X) & \giv \\ %1
		    \fa \fh \exists X p(X) & \ass \\ %2
		      \fa \fa \fh p(a) & \ass \\ %3
		        \fa \fa \fa \fh \exists X p(X) & \ass \\ %4
		        \fa \fa \fa \fa \lnot p(a) & \forallE{4} \\ %5
		      \fa \fa \fa \lnot \exists X p(X) & \raa{4}{3}{5} \\%6
        \fa \fa \lnot \exists X p(X) & \existsE{2}{3}{6} \\ %7
		  \fa \lnot \exists X p(X) & \existsE{2}{2}{7} \\ %8
      
		\end{fitch}
	\end{equation*}
	
	\subsection{DeMorgan's rule: \texorpdfstring{ $ \lnot \forall X p(X) \equiv \exists X \lnot p(X) $}{DeMorgan}}
  $ \lnot \forall X p(X) \vdash \exists X \lnot p(X) $
	  \begin{equation*}
		  \begin{fitch}
		    
	    \end{fitch}
  	\end{equation*}
  
  $ \exists X \lnot p(X) \vdash \lnot \forall X p(X) $
    \begin{equation*}
  	  \begin{fitch}

      \end{fitch}
  	\end{equation*}
\end{document}